minuska/theories/prelude.v
@@ -162,3 +162,46 @@ Proof.
     { reflexivity. }
     { inversion IH. }
 Qed.
+
+
+Lemma rev_list_ind_T [A : Type] :
+    forall P:list A-> Type,
+    P [] ->
+    (forall (a:A) (l:list A), P (rev l) -> P (rev (a :: l))) ->
+    forall l:list A, P (rev l). 
+Proof.
+    intros P ? ? l; induction l; auto.
+Qed.
+
+Lemma rev_ind_T :
+∀ [A : Type] (P : list A → Type),
+  P [] → (∀ (x : A) (l : list A), P l → P (l ++ [x])) → ∀ l : list A, P l
+.
+Proof.
+    intros A P ? ? l. rewrite <- (rev_involutive l).
+    apply (rev_list_ind_T P); cbn; auto.
+Qed.
+
+
+Definition analyze_list_from_end {A : Type} (l : list A)
+    : (l = nil) + ( ({ l' : list A & { x : A & l = l'++[x] } }))
+.
+Proof.
+    induction l.
+    {
+        left. reflexivity.
+    }
+    {
+        right.
+        destruct IHl as [IHl|IHl].
+        {
+            subst. exists []. exists a. reflexivity.
+        }
+        {
+            destruct IHl as [l' [x Hl']].
+            subst.
+            exists (a::l'). exists x. simpl. reflexivity.
+        }
+    }
+Qed.
+
